Integrated statistics module

statistics.dfy
@@ -1,106 +1,139 @@
-module Statistics {
-
-  
-  predicate Sorted(s: seq<real>)
-  {
-    forall i :: 0 <= i && i + 1 < |s| ==> s[i] <= s[i+1]
-  }
- // This is the join function which combines the 2 sorted parts
-  function merge_join(first: seq<real>, second: seq<real>) : seq<real>
-    decreases |first| + |second|
-  {
-    if |first| == 0 then second
-    else if |second| == 0 then first
-    else if first[0] <= second[0]
-         then [first[0]] + merge_join(first[1..], second)
-         else [second[0]] + merge_join(first, second[1..])
-  }
-// This is the split function which splits the sequence into 2 parts
-  function merge_split(s: seq<real>) : seq<real>
-    decreases |s|
-  {
-    if |s| <= 1 then s
-    else
-      var mid := |s| / 2;
-      merge_join(merge_split(s[..mid]), merge_split(s[mid..]))
-  }
-
-  lemma merge_join_Length(first: seq<real>, second: seq<real>)
-    ensures |merge_join(first,second)| == |first| + |second|
-    decreases |first| + |second|
-  {
-    if |first| == 0 || |second| == 0 { }
-    else if first[0] <= second[0] {
-      merge_join_Length(first[1..], second);
-    } else {
-      merge_join_Length(first, second[1..]);
-    }
-  }
-
-  lemma merge_split_Length(s: seq<real>)
-    ensures |merge_split(s)| == |s|
-    decreases |s|
-  {
-    if |s| <= 1 { }
-    else {
-      var mid := |s| / 2;
-      merge_split_Length(s[..mid]);
-      merge_split_Length(s[mid..]);
-      merge_join_Length(merge_split(s[..mid]), merge_split(s[mid..]));
-    }
-  }
-
-  lemma merge_join_sorted(first: seq<real>, second: seq<real>)
-    requires Sorted(first) && Sorted(second)
-    ensures Sorted(merge_join(first,second))
-    decreases |first| + |second|
-  {
-    if |first| == 0 || |second| == 0 {
-    } else if first[0] <= second[0] {
-      merge_join_sorted(first[1..], second);
-      if |first| >= 2 {
-        assert first[0] <= first[1];
-      } else {
-        assert first[0] <= second[0];
-      }
-    } else {
-      merge_join_sorted(first, second[1..]);
-      if |second| >= 2 {
-        assert second[0] <= second[1];
-      } else {
-        assert second[0] <= first[0];
-      }
-    }
-  }
-
-  lemma merge_split_Sorted(s: seq<real>)
-    ensures Sorted(merge_split(s))
-    decreases |s|
-  {
-    if |s| <= 1 { }
-    else {
-      var mid := |s| / 2;
-      merge_split_Sorted(s[..mid]);
-      merge_split_Sorted(s[mid..]);
-      merge_join_sorted(merge_split(s[..mid]), merge_split(s[mid..]));
-    }
-  }
-
-  
-
-  method Median(s: seq<real>) returns (m: real)
-  requires |s| > 0
-  ensures (|merge_split(s)| % 2 == 1 ==> 
-             m == merge_split(s)[|merge_split(s)|/2])
-  ensures (|merge_split(s)| % 2 == 0 && |merge_split(s)| >= 2 ==> 
-             m == (merge_split(s)[|merge_split(s)|/2 - 1] + merge_split(s)[|merge_split(s)|/2]) / 2.0)
-{
-  var t := merge_split(s);
- merge_split_Length(s);                         
-  if |t| % 2 == 1 {
-    m := t[|t|/2];
-  } else {
-    m := (t[|t|/2 - 1] + t[|t|/2]) / 2.0;
-  }
+module ExternalMath {
+  function {:extern} Sqrt(x: real): real
+    requires x >= 0.0
+    ensures Sqrt(x) >= 0.0
+    ensures var result := Sqrt(x); result * result <= x + 0.0000001
+    ensures var result := Sqrt(x); result * result >= x - 0.0000001
 }
+
+module Statistics {
+  import opened ExternalMath
+  import opened Std.Collections.Seq
+
+  // A function to sum the elements of a sequence
+  function Sum(s: seq<real>): real
+  {
+    if |s| == 0 then
+      0.0
+    else
+      s[0] + Sum(s[1..])
+  }
+
+  // A function to compute the mean (average) as a real number
+  function Mean(s: seq<real>): real
+    requires |s| > 0
+    ensures Mean(s) == Sum(s) / (|s| as real)
+  {
+    Sum(s) / (|s| as real)
+  }
+
+  // A helper function to calculate the sum of squared differences from a given mean
+  function SumSquaredDifferences(s: seq<real>, avg: real): real
+    ensures SumSquaredDifferences(s, avg) >= 0.0
+  {
+    if |s| == 0 then
+      0.0
+    else
+      var diff := s[0] - avg;
+      diff * diff + SumSquaredDifferences(s[1..], avg)
+  }
+  // Function to calculate the absolute value of a real number
+  function RealAbs(x: real): real
+    ensures RealAbs(x) >= 0.0
+    ensures RealAbs(x) == x || RealAbs(x) == -x
+  {
+    if x >= 0.0 then x else -x
+  }
+  // Function to check if two real numbers are close within a given tolerance.
+  function AreNear(a: real, b: real, epsilon: real): bool
+    requires epsilon >= 0.0
+    ensures AreNear(a, b, epsilon) == (RealAbs(a - b) <= epsilon)
+  {
+    RealAbs(a - b) <= epsilon
+  }
+
+  // A function to calculate Population Variance
+  function VariancePopulation(s: seq<real>): real
+    requires |s| > 0
+    ensures VariancePopulation(s) >= 0.0
+    ensures VariancePopulation(s) == SumSquaredDifferences(s, Mean(s)) / (|s| as real)
+  {
+    var avg := Mean(s);
+    SumSquaredDifferences(s, avg) / (|s| as real)
+  }
+
+  // A function to calculate Sample Variance
+  function VarianceSample(s: seq<real>): real
+    requires |s| > 1
+    ensures VarianceSample(s) >= 0.0
+  {
+    var avg := Mean(s);
+    (SumSquaredDifferences(s, avg)) / ((|s| - 1) as real)
+  }
+
+  // A function to calculate Population Standard Deviation
+  function StdDevPopulation(s: seq<real>): real
+    requires |s| > 0
+    ensures StdDevPopulation(s) >= 0.0
+  {
+    ExternalMath.Sqrt(VariancePopulation(s))
+  }
+
+  // A function to calculate Sample Standard Deviation
+  function StdDevSample(s: seq<real>): real
+    requires |s| > 1
+    ensures StdDevSample(s) >= 0.0
+  {
+    ExternalMath.Sqrt(VarianceSample(s))
+  }
+
+
+
+  // Median of a non-empty sequence of real numbers
+  function Median(a: seq<real>): real
+    requires |a| > 0
+    ensures var sorted := MergeSortBy((x: real, y: real) => x <= y, a);
+            if |a| % 2 == 1 then
+              Median(a) == sorted[|a|/2]
+            else
+              Median(a) == (sorted[|a|/2 - 1] + sorted[|a|/2]) / 2.0
+  {
+    // Existing merge sort utilized
+    var sorted := MergeSortBy((x: real, y: real) => x <= y, a);
+    if |a| % 2 == 1 then
+      sorted[|a|/2]
+    else
+      (sorted[|a|/2 - 1] + sorted[|a|/2]) / 2.0
+  }
+
+  //The function for keeping a Count of the elements. This will be recursively called
+  function Count(s: seq<real>, v: real): nat
+    decreases s
+  {
+    if |s| == 0 then 0
+    else if s[0] == v then 1 + Count(s[1..], v)
+    else Count(s[1..], v)
+  }
+
+  // The function for calcluating mode
+  function Mode(s: seq<real>): real
+    requires |s| > 0
+    ensures Mode(s) in s
+    ensures (forall x :: x in s ==> Count(s, x) <= Count(s, Mode(s)))
+  {
+    if |s| == 1 then s[0]
+    else if Count(s, s[0]) >= Count(s[1..], Mode(s[1..])) then s[0]
+    else Mode(s[1..])
+  }
+
+  // The function for calcluating range for a sequence which is the max element - min element
+  function Range(s: seq<real>): real
+    requires |s| > 0
+    ensures Range(s) >= 0.0
+  {
+    var sorted := MergeSortBy((x: real, y: real) => x <= y, s);
+    sorted[|s| - 1] - sorted[0]
+  }
+
+
 }
